module Algebra where

open import Subset
open import Logic
open import ZAxioms

infix 6 _âˆª_
infix 6 _-_

-- Properties involving operations between sets, algebra of sets.

-- In this module some properties involving union, difference
-- and intersection of set are proved.

-- First, some properties of the union between sets, justified by the
-- union axiom.

_âˆª_ : ğ“¢ â†’ ğ“¢ â†’ ğ“¢
x âˆª y = projâ‚ (union x y)
{-# ATP definition _âˆª_ #-}

-- Theorem 20, p. 27 (Suppes 1960)
âˆª-d : (x y : ğ“¢) â†’ âˆ€ {z} â†’ z âˆˆ x âˆª y â‡” z âˆˆ x âˆ¨ z âˆˆ y
âˆª-d x y = projâ‚‚ _ (union x y)

-- âˆ§-projections of past theorem for convenience.
âˆª-dâ‚ : (A B : ğ“¢) â†’ âˆ€ {x} â†’ x âˆˆ (A âˆª B) â†’ x âˆˆ A âˆ¨ x âˆˆ B
âˆª-dâ‚ A B = âˆ§-projâ‚ (âˆª-d A B)

âˆª-dâ‚‚ : (A B : ğ“¢) â†’ âˆ€ {x} â†’ x âˆˆ A âˆ¨ x âˆˆ B â†’ x âˆˆ (A âˆª B)
âˆª-dâ‚‚ A B = âˆ§-projâ‚‚ (âˆª-d A B)

-- Theorem 21, p. 27 (Suppes 1960)
AâˆªBâ‰¡BâˆªA : (A B : ğ“¢) â†’ A âˆª B â‰¡ B âˆª A
AâˆªBâ‰¡BâˆªA A B = equalitySubset (A âˆª B) (B âˆª A) (pâ‚ , pâ‚‚)
  where
  pâ‚ : (x : ğ“¢) â†’ x âˆˆ (A âˆª B) â†’ x âˆˆ (B âˆª A)
  pâ‚ x xâ‚ = âˆª-dâ‚‚ B A (âˆ¨-sym _ _ (âˆª-dâ‚ A B xâ‚))
  pâ‚‚ : (x : ğ“¢) â†’ x âˆˆ (B âˆª A) â†’ x âˆˆ (A âˆª B)
  pâ‚‚ x xâ‚ = âˆª-dâ‚‚ A B (âˆ¨-sym _ _ (âˆª-dâ‚ B A xâ‚))

-- Theorem 23, p. 27 (Suppes 1960)
AâˆªAâ‰¡A : (A : ğ“¢) â†’ A âˆª A â‰¡ A
AâˆªAâ‰¡A A = equalitySubset (A âˆª A) A (pâ‚ , pâ‚‚)
  where
  pâ‚ : (x : â€„ğ“¢) â†’ x âˆˆ (A âˆª A) â†’ x âˆˆ A
  pâ‚ x xâ‚ = âˆ¨-idem _ (âˆª-dâ‚ A A xâ‚)
  pâ‚‚ : (x : ğ“¢) â†’ x âˆˆ A â†’ x âˆˆ (A âˆª A)
  pâ‚‚ x xâ‚ = âˆª-dâ‚‚ A A (injâ‚ xâ‚)

-- Theorem 25, p. 27 (Suppes 1960)
âˆª-prop : (A B : ğ“¢) â†’ A âŠ† A âˆª B
âˆª-prop A B t x = âˆª-dâ‚‚ _ _ (injâ‚ x)

âŠ†âˆª : (x A B : ğ“¢) â†’ x âŠ† A âˆ§ x âŠ† B â†’ x âŠ† A âˆª B
âŠ†âˆª x A B (xâ‚ , xâ‚‚) t xâ‚ƒ = trans-âŠ† _ _ _ (xâ‚ , (âˆª-prop _ _)) _ xâ‚ƒ

âˆª-propâ‚‚ : (x A B : ğ“¢) â†’ x âŠ† A âˆ¨ x âŠ† B â†’ x âŠ† A âˆª B
âˆª-propâ‚‚ x A B (injâ‚ xâ‚) t xâ‚‚ = âˆª-dâ‚‚ _ _ (injâ‚ (xâ‚ _ xâ‚‚))
âˆª-propâ‚‚ x A B (injâ‚‚ xâ‚) t xâ‚‚ = âˆª-dâ‚‚ _ _ (injâ‚‚ (xâ‚ _ xâ‚‚))

âˆª-propâ‚ƒ : (A B : ğ“¢) â†’ B âŠ† A âˆª B
âˆª-propâ‚ƒ A B t x = âˆª-dâ‚‚ _ _ (injâ‚‚ x)

-- Theorem 27, p. 27 (Suppes 1960)
âˆª-propâ‚„ : (x y A : ğ“¢) â†’ x âŠ† A â†’ y âŠ† A â†’ x âˆª y âŠ† A
âˆª-propâ‚„ x y A xâŠ†A yâŠ†A t tâˆˆxâˆªy = âˆ¨-idem _ pâ‚‚
  where
  pâ‚ : t âˆˆ x âˆ¨ t âˆˆ y
  pâ‚ = âˆª-dâ‚ _ _ tâˆˆxâˆªy
  pâ‚‚ : t âˆˆ A âˆ¨ t âˆˆ A
  pâ‚‚ = âˆ¨-propâ‚… pâ‚ (xâŠ†A _) (yâŠ†A _)

-- Properties about the intersection opertaion. Its existence is justified
-- as an axiom derived from the sub axiom schema.

-- Instantiation of the subset axiom schema needed for justifiying
-- the operation.
subâ‚‚ : (x y : ğ“¢) â†’ âˆƒ (Î» B â†’ {z : ğ“¢} â†’ (z âˆˆ B â‡” z âˆˆ x âˆ§ z âˆˆ y))
subâ‚‚ x y = sub (Î» z â†’ z âˆˆ y) x

-- Theorem 12, p.25 (Suppes 1960)
âˆ©-def : (x y : ğ“¢) â†’ âˆ€ {z} â†’ z âˆˆ x âˆ© y â‡” z âˆˆ x âˆ§ z âˆˆ y
âˆ©-def x y = projâ‚‚ _ (subâ‚‚ x y)

-- Projections of âˆ©-def, useful for avoiding repeating this
-- projections later.
âˆ©-dâ‚ : (x A B : ğ“¢)  â†’ x âˆˆ (A âˆ© B) â†’ x âˆˆ A âˆ§ x âˆˆ B
âˆ©-dâ‚ x A B = âˆ§-projâ‚ (âˆ©-def A B)

âˆ©-dâ‚‚ : (x A B : ğ“¢) â†’ x âˆˆ A âˆ§ x âˆˆ B â†’ x âˆˆ (A âˆ© B)
âˆ©-dâ‚‚ x A B = âˆ§-projâ‚‚ (âˆ©-def A B)

-- Theorem 13, p.26 (Suppes 1960)
âˆ©-sym : (A B : ğ“¢) â†’ A âˆ© B â‰¡ B âˆ© A
âˆ©-sym A B = equalitySubset (A âˆ© B) (B âˆ© A) (pâ‚ , pâ‚‚)
  where
  pâ‚ : (x : ğ“¢) â†’ x âˆˆ A âˆ© B â†’ x âˆˆ B âˆ© A
  pâ‚ x xâˆˆAâˆ©B = âˆ©-dâ‚‚ x B A (xâˆˆB , xâˆˆA)
    where
    xâˆˆA : x âˆˆ A
    xâˆˆA = âˆ§-projâ‚ (âˆ©-dâ‚ x A B xâˆˆAâˆ©B)
    xâˆˆB : x âˆˆ B
    xâˆˆB = âˆ§-projâ‚‚ (âˆ©-dâ‚ x A B xâˆˆAâˆ©B)
  pâ‚‚ : (x : â€¯ğ“¢) â†’ x âˆˆ B âˆ© A â†’ x âˆˆ A âˆ© B
  pâ‚‚ x xâˆˆBâˆ©A = âˆ©-dâ‚‚ x A B (xâˆˆA , xâˆˆB)
    where
    xâˆˆA : x âˆˆ A
    xâˆˆA = âˆ§-projâ‚‚ (âˆ©-dâ‚ x B A xâˆˆBâˆ©A)
    xâˆˆB : x âˆˆ B
    xâˆˆB = âˆ§-projâ‚ (âˆ©-dâ‚ x B A xâˆˆBâˆ©A)

-- Theorem 14, p. 26 (Suppes 1960).
âˆ©-dist : (A B C : ğ“¢) â†’ (A âˆ© B) âˆ© C â‰¡ A âˆ© (B âˆ© C)
âˆ©-dist A B C = equalitySubset ((A âˆ© B) âˆ© C) (A âˆ© (B âˆ© C)) (pâ‚ , pâ‚‚)
  where
  pâ‚ : (x : ğ“¢) â†’ x âˆˆ (A âˆ© B) âˆ© C â†’ x âˆˆ A âˆ© (B âˆ© C)
  pâ‚ x xâ‚ = âˆ©-dâ‚‚ x A (B âˆ© C) (xâˆˆA , xâˆˆBâˆ©C)
    where
    xâˆˆBâˆ©C : x âˆˆ B âˆ© C
    xâˆˆBâˆ©C = âˆ©-dâ‚‚ x B C (xâˆˆB , xâˆˆC)
      where
      xâˆˆAâˆ©B : x âˆˆ A âˆ© B
      xâˆˆAâˆ©B = âˆ§-projâ‚ (âˆ©-dâ‚ x (A âˆ© B) _ xâ‚)
      xâˆˆB : x âˆˆ B
      xâˆˆB = âˆ§-projâ‚‚ (âˆ©-dâ‚ x _ B xâˆˆAâˆ©B)
      xâˆˆC : x âˆˆ C
      xâˆˆC = âˆ§-projâ‚‚ (âˆ©-dâ‚ x _ C xâ‚)
    xâˆˆA : x âˆˆ A
    xâˆˆA = âˆ§-projâ‚ (âˆ©-dâ‚ x A _ xâˆˆAâˆ©B)
      where
      xâˆˆAâˆ©B : x âˆˆ A âˆ© B
      xâˆˆAâˆ©B = âˆ§-projâ‚ (âˆ©-dâ‚ x (A âˆ© B) _ xâ‚)
  pâ‚‚ : (x : ğ“¢) â†’ x âˆˆ A âˆ© (B âˆ© C) â†’ x âˆˆ (A âˆ© B) âˆ© C
  pâ‚‚ x xâ‚ = âˆ©-dâ‚‚ x (A âˆ© B) C (xâˆˆAâˆ©B , xâˆˆC)
    where
    xâˆˆAâˆ©B : x âˆˆ A âˆ© B
    xâˆˆAâˆ©B = âˆ©-dâ‚‚ x A B (xâˆˆA , xâˆˆB)
      where
      xâˆˆA : x âˆˆ A
      xâˆˆA = âˆ§-projâ‚ (âˆ©-dâ‚ x A _ xâ‚)
      xâˆˆBâˆ©C : x âˆˆ B âˆ© C
      xâˆˆBâˆ©C = âˆ§-projâ‚‚ (âˆ©-dâ‚ x _ (B âˆ© C) xâ‚)
      xâˆˆB : x âˆˆ B
      xâˆˆB = âˆ§-projâ‚ (âˆ©-dâ‚ x B _ xâˆˆBâˆ©C)
    xâˆˆC : x âˆˆ C
    xâˆˆC = âˆ§-projâ‚‚ (âˆ©-dâ‚ x _ C xâˆˆBâˆ©C)
      where
      xâˆˆBâˆ©C : x âˆˆ B âˆ© C
      xâˆˆBâˆ©C = âˆ§-projâ‚‚ (âˆ©-dâ‚ x _ (B âˆ© C) xâ‚)

-- Theorem 15, p. 26 (Suppes).
âˆ©-itself : (A : ğ“¢) â†’ A âˆ© A â‰¡ A
âˆ©-itself A = equalitySubset (A âˆ© A) A (pâ‚ , pâ‚‚)
  where
  pâ‚ : (x : ğ“¢) â†’ x âˆˆ A âˆ© A â†’ x âˆˆ A
  pâ‚ x xâ‚ = âˆ§-projâ‚ (âˆ©-dâ‚ _ A _ xâ‚)
  pâ‚‚ : (x : â€„ğ“¢) â†’ x âˆˆ A â†’ x âˆˆ A âˆ© A
  pâ‚‚ x xâ‚ = âˆ©-dâ‚‚ _ A A (xâ‚ , xâ‚)

-- Theorem 17, p. 26 (Suppes 1960).
Aâˆ©BâŠ†A : (A B : ğ“¢) â†’ A âˆ© B âŠ† A
Aâˆ©BâŠ†A A B _ p = âˆ§-projâ‚ (âˆ©-dâ‚ _ A _ p)

-- Properties involving the difference between sets. The existence of this
-- sets is also justified as an instance of the subset axiom schema.

-- Instantiation of the subset schema that will justify the operation
-- of difference between sets.
subâ‚ƒ : (x y : ğ“¢) â†’ âˆƒ (Î» B â†’ {z : ğ“¢} â†’ (z âˆˆ B â‡” z âˆˆ x âˆ§ z âˆ‰ y))
subâ‚ƒ x y = sub (Î» z â†’ z âˆ‰ y) x

_-_ : ğ“¢ â†’ ğ“¢ â†’ ğ“¢
x - y = projâ‚ (subâ‚ƒ x y)

-- Theorem 31, p.28 (Suppes 1960).
dif-def : (x y : ğ“¢) â†’ âˆ€ {z} â†’ z âˆˆ (x - y) â‡” z âˆˆ x âˆ§ z âˆ‰ y
dif-def x y = projâ‚‚ _ (subâ‚ƒ x y)

-- Again both âˆ§-projections of the past theorem.
dif-dâ‚ : (A B z : ğ“¢) â†’ z âˆˆ A - B â†’ z âˆˆ A âˆ§ z âˆ‰ B
dif-dâ‚ A B z = âˆ§-projâ‚ (dif-def A B)

dif-dâ‚‚ : (A B z : ğ“¢) â†’ z âˆˆ A âˆ§ z âˆ‰ B â†’ z âˆˆ A - B
dif-dâ‚‚ A B z = âˆ§-projâ‚‚ (dif-def A B)

-- Theorem 33, p. 29 (Suppes 1960).
âˆ©- : (A B : ğ“¢) â†’ A âˆ© (A - B) â‰¡ A - B
âˆ©- A B = equalitySubset (A âˆ© (A - B)) (A - B) (pâ‚ , pâ‚‚)
  where
  pâ‚ : (x : ğ“¢) â†’ x âˆˆ A âˆ© (A - B) â†’ x âˆˆ A - B
  pâ‚ x xâˆˆâˆ©- = dif-dâ‚‚ A B x (xâˆˆA , xâˆ‰B)
    where
    xâˆˆA : x âˆˆ A
    xâˆˆA = âˆ§-projâ‚ (âˆ©-dâ‚ x A _ xâˆˆâˆ©-)
    xâˆˆA-B : x âˆˆ A - B
    xâˆˆA-B = âˆ§-projâ‚‚ (âˆ©-dâ‚ x _ (A - B) xâˆˆâˆ©-)
    xâˆ‰B : x âˆ‰ B
    xâˆ‰B = âˆ§-projâ‚‚ (dif-dâ‚ A B x xâˆˆA-B)
  pâ‚‚ : (x : ğ“¢) â†’ x âˆˆ A - B â†’ x âˆˆ A âˆ© (A - B)
  pâ‚‚ x xâˆˆA-B = âˆ©-dâ‚‚ x A (A - B) ((âˆ§-projâ‚ (dif-dâ‚ A B x xâˆˆA-B)) , xâˆˆA-B)
