---------------------------------------
-- Pairs of sets
---------------------------------------

{-# OPTIONS --allow-unsolved-meta #-}

module Pairs where

-- Everything involving pairs, be them unordered
-- or ordered pairs. Also the definition of power set
-- and cartesian product between sets.

open import Logic
open import Algebra
open import Subset
open import ZAxioms

-- Pairs, justified by the pair axiom

_â‚š_ : ğ“¢ â†’ ğ“¢ â†’ ğ“¢
x â‚š y = projâ‚ (pair x y)

pair-d : (x y : ğ“¢) â†’ âˆ€ {z} â†’ z âˆˆ x â‚š y â‡” (z â‰¡ x âˆ¨ z â‰¡ y)
pair-d x y = projâ‚‚ _ (pair x y)

-- Both âˆ§-projections
pair-dâ‚ : (x y : ğ“¢) â†’ âˆ€ {z} â†’ z âˆˆ x â‚š y â†’ (z â‰¡ x âˆ¨ z â‰¡ y)
pair-dâ‚ x y = âˆ§-projâ‚ (pair-d x y)

pair-dâ‚‚ : (x y : ğ“¢) â†’ âˆ€ {z} â†’ (z â‰¡ x âˆ¨ z â‰¡ y) â†’ z âˆˆ x â‚š y
pair-dâ‚‚ x y = âˆ§-projâ‚‚ (pair-d x y)

pair-pâ‚ : (x y : ğ“¢) â†’ x â‚š y â‰¡ y â‚š x
pair-pâ‚ x y = equalitySubset (x â‚š y) (y â‚š x) (pâ‚ , pâ‚‚)
  where
  pâ‚ : (z : ğ“¢) â†’ z âˆˆ x â‚š y â†’ z âˆˆ y â‚š x
  pâ‚ z zâˆˆx,y = pair-dâ‚‚ y x (âˆ¨-sym _ _ (pair-dâ‚ x y zâˆˆx,y))

  pâ‚‚ : (z : ğ“¢) â†’ z âˆˆ y â‚š x â†’ z âˆˆ x â‚š y
  pâ‚‚ z zâˆˆy,x = pair-dâ‚‚ x y (âˆ¨-sym _ _ (pair-dâ‚ y x zâˆˆy,x))

singleton : ğ“¢ â†’ ğ“¢
singleton x = x â‚š x

singletonp : (x : ğ“¢) â†’ âˆ€ {z} â†’ z âˆˆ singleton x â†’ z â‰¡ x
singletonp x xâ‚ = âˆ¨-idem _ (pair-dâ‚ x x xâ‚)

singletonpâ‚‚ : (x : ğ“¢) â†’ x âˆˆ singleton x
singletonpâ‚‚ x = pair-dâ‚‚ x x (injâ‚ refl)

singletonpâ‚ƒ : (x : ğ“¢) â†’ âˆ€ {y} â†’ x â‰¡ y â†’ x âˆˆ singleton y
singletonpâ‚ƒ x xâ‰¡y = pair-dâ‚‚ _ _ (injâ‚ xâ‰¡y)

singletonpâ‚„ : (x y : ğ“¢) â†’ x âˆˆ singleton y â†’ x âˆ© singleton y â‰¡ âˆ…
singletonpâ‚„ x y h = {!!}
  where
  pâ‚ : x â‰¡ y
  pâ‚ = singletonp _ h

  pâ‚‚ : x âˆ© singleton x â‰¡ âˆ…
  pâ‚‚ = {!!}

pair-prop-helperâ‚ : {a b c : ğ“¢} â†’ a â‰¡ b âˆ¨ a â‰¡ c â†’ a â‰¢ b â†’ a â‰¡ c
pair-prop-helperâ‚ (injâ‚ aâ‰¡b) h = âŠ¥-elim (h aâ‰¡b)
pair-prop-helperâ‚ (injâ‚‚ refl) _ = refl

pair-prop-helperâ‚‚ : {a b : ğ“¢} â†’ a â‰¢ b â†’ b â‰¢ a
pair-prop-helperâ‚‚ h bâ‰¡a = h (sym _ _ bâ‰¡a)

-- Theorem 44, p. 31 (Suppes, 1972).
pair-prop : (x y u v : ğ“¢) â†’ x â‚š y â‰¡ u â‚š v â†’ (u â‰¡ x âˆ§ v â‰¡ y) âˆ¨ (v â‰¡ x âˆ§ u â‰¡ y)
pair-prop x y u v eq = âˆ¨-e _ _ _ (pem (x â‰¡ y)) h-xâ‰¡y h-xâ‰¢y
  where
  uâˆˆu,v : u âˆˆ (u â‚š v)
  uâˆˆu,v = âˆ¨-propâ‚ (pair-dâ‚‚ u v) refl

  uâˆˆx,y : u âˆˆ (x â‚š y)
  uâˆˆx,y = memberEq u (u â‚š v) (x â‚š y) (uâˆˆu,v , (sym _ _ eq))

  disjâ‚ : u â‰¡ x âˆ¨ u â‰¡ y
  disjâ‚ = pair-dâ‚ _ _ uâˆˆx,y

  vâˆˆu,v : v âˆˆ (u â‚š v)
  vâˆˆu,v = âˆ¨-propâ‚‚ (pair-dâ‚‚ u v) refl

  vâˆˆx,y : v âˆˆ (x â‚š y)
  vâˆˆx,y = memberEq v (u â‚š v) (x â‚š y) (vâˆˆu,v , (sym _ _ eq))

  disjâ‚‚ : v â‰¡ x âˆ¨ v â‰¡ y
  disjâ‚‚ = pair-dâ‚ _ _ vâˆˆx,y

  xâˆˆx,y : x âˆˆ (x â‚š y)
  xâˆˆx,y = âˆ¨-propâ‚ (pair-dâ‚‚ x y) refl

  xâˆˆu,v : x âˆˆ (u â‚š v)
  xâˆˆu,v = memberEq x (x â‚š y) (u â‚š v) (xâˆˆx,y , eq)

  disjâ‚ƒ : x â‰¡ u âˆ¨ x â‰¡ v
  disjâ‚ƒ = pair-dâ‚ _ _ xâˆˆu,v

  yâˆˆx,y : y âˆˆ (x â‚š y)
  yâˆˆx,y = âˆ¨-propâ‚‚ (pair-dâ‚‚ x y) refl

  yâˆˆu,v : y âˆˆ (u â‚š v)
  yâˆˆu,v = memberEq y (x â‚š y) (u â‚š v) (yâˆˆx,y , eq)

  disjâ‚„ : y â‰¡ u âˆ¨ y â‰¡ v
  disjâ‚„ = pair-dâ‚ _ _ yâˆˆu,v

  h-xâ‰¡y : x â‰¡ y â†’ (u â‰¡ x âˆ§ v â‰¡ y) âˆ¨ (v â‰¡ x âˆ§ u â‰¡ y)
  h-xâ‰¡y eqâ‚‚ = injâ‚ (xâ‰¡u , vâ‰¡y)
    where
    xâ‰¡u : u â‰¡ x
    xâ‰¡u = âˆ¨-idem _ disj-aux
      where
      disj-aux : u â‰¡ x âˆ¨ u â‰¡ x
      disj-aux = subs _ (sym _ _ eqâ‚‚) disjâ‚

    vâ‰¡y : v â‰¡ y
    vâ‰¡y = âˆ¨-idem _ disj-aux
      where
      disj-aux : v â‰¡ y âˆ¨ v â‰¡ y
      disj-aux = subs _ eqâ‚‚ disjâ‚‚

  h-xâ‰¢y : x â‰¢ y â†’ (u â‰¡ x âˆ§ v â‰¡ y) âˆ¨ (v â‰¡ x âˆ§ u â‰¡ y)
  h-xâ‰¢y Â¬eq = âˆ¨-e _ _ _ (pem (x â‰¡ u)) hâ‚ hâ‚‚
    where
    hâ‚ : x â‰¡ u â†’ (u â‰¡ x âˆ§ v â‰¡ y) âˆ¨ (v â‰¡ x âˆ§ u â‰¡ y)
    hâ‚ xâ‰¡u = âˆ¨-e _ _ _ (pem (y â‰¡ u)) hâ‚â‚ hâ‚â‚‚
      where
      hâ‚â‚ : y â‰¡ u â†’ (u â‰¡ x âˆ§ v â‰¡ y) âˆ¨ (v â‰¡ x âˆ§ u â‰¡ y)
      hâ‚â‚ yâ‰¡u = âŠ¥-elim (Â¬eq (trans xâ‰¡u (sym _ _ yâ‰¡u)))

      hâ‚â‚‚ : y â‰¢ u â†’ (u â‰¡ x âˆ§ v â‰¡ y) âˆ¨ (v â‰¡ x âˆ§ u â‰¡ y)
      hâ‚â‚‚ h = injâ‚ (sym _ _ xâ‰¡u , sym _ _ (pair-prop-helperâ‚ disjâ‚„ h))

    hâ‚‚ : x â‰¢ u â†’ (u â‰¡ x âˆ§ v â‰¡ y) âˆ¨ (v â‰¡ x âˆ§ u â‰¡ y)
    hâ‚‚ h = injâ‚‚ (sym _ _ (pair-prop-helperâ‚ disjâ‚ƒ h)
                ,
                (pair-prop-helperâ‚ disjâ‚ (pair-prop-helperâ‚‚ h)))

-- Theorem 45, p. 32 (Suppes 1960).
singleton-eq : (x y : ğ“¢) â†’ singleton x â‰¡ singleton y â†’ x â‰¡ y
singleton-eq x y eq = sym _ _ (âˆ§-projâ‚ (âˆ¨-idem _ aux))
  where
  aux : ((y â‰¡ x) âˆ§ (y â‰¡ x)) âˆ¨ ((y â‰¡ x) âˆ§ (y â‰¡ x))
  aux = pair-prop x x y y eq

singleton-âŠ† : (x A : ğ“¢) â†’ x âˆˆ A â†’ singleton x âŠ† A
singleton-âŠ† x A xâˆˆA t tâˆˆxâ‚› = subs _ (sym _ _ (singletonp _ tâˆˆxâ‚›)) xâˆˆA

prop-pâ‚‚ : (y z : ğ“¢) â†’ y â‚š z â‰¡ singleton y âˆª singleton z
prop-pâ‚‚ y z = equalitySubset _ _ (pâ‚ , pâ‚‚)
  where
  pâ‚ : (x : ğ“¢) â†’ x âˆˆ y â‚š z â†’ x âˆˆ singleton y âˆª singleton z
  pâ‚ _ h = âˆª-dâ‚‚ _ _ (âˆ¨-propâ‚… (pair-dâ‚ _ _ h) (singletonpâ‚ƒ _) (singletonpâ‚ƒ _))

  pâ‚‚ : (x : ğ“¢) â†’ x âˆˆ singleton y âˆª singleton z â†’ x âˆˆ y â‚š z
  pâ‚‚ x h = pair-dâ‚‚ _ _ (âˆ¨-propâ‚… (âˆª-dâ‚ _ _ h) (singletonp _) (singletonp _))

-- Ordered pairs

_â‚’_ : ğ“¢ â†’ ğ“¢ â†’ ğ“¢
x â‚’ y = singleton x â‚š (x â‚š y)

-- Just an abvreviation for next theorem
abvâ‚ : ğ“¢ â†’ ğ“¢ â†’ ğ“¢ â†’ ğ“¢ â†’ Set
abvâ‚ u x v y = (u â‚š u â‰¡ x â‚š x âˆ§ u â‚š v â‰¡ x â‚š y) âˆ¨ (u â‚š v â‰¡ x â‚š x âˆ§ u â‚š u â‰¡ x â‚š y)

-- Theorem 46, p. 32 (Suppes).
ord-p : (x y u v : ğ“¢) â†’ x â‚’ y â‰¡ u â‚’ v â†’ x â‰¡ u âˆ§ y â‰¡ v
ord-p x y u v eq = âˆ¨-e _ _ _ aux aâ†’c bâ†’c
  where
  aux : abvâ‚ u x v y
  aux = pair-prop _ _ _ _ eq

  aâ†’c : singleton u â‰¡ singleton x âˆ§ u â‚š v â‰¡ x â‚š y â†’ x â‰¡ u âˆ§ y â‰¡ v
  aâ†’c (eqâ‚š , eqâ‚›) = xâ‰¡u , yâ‰¡v
    where
    xâ‰¡u : x â‰¡ u
    xâ‰¡u = singleton-eq _ _ (sym _ _ eqâ‚š)

    yâ‰¡v : y â‰¡ v
    yâ‰¡v = {!!}
  bâ†’c : u â‚š v â‰¡ singleton x âˆ§ singleton u â‰¡ x â‚š y â†’ x â‰¡ u âˆ§ y â‰¡ v
  bâ†’c xâ‚ = {!!}

-- Power sets

ğ“Ÿ_ : ğ“¢ â†’ ğ“¢
ğ“Ÿ x = projâ‚ (pow x)

-- Theorem 86, p. 47 (Suppes 1960)
ğ“Ÿ-d : (x : ğ“¢) â†’ âˆ€ {z} â†’ z âˆˆ (ğ“Ÿ x) â‡” z âŠ† x
ğ“Ÿ-d x = projâ‚‚ _ (pow x)

-- Both projections.
ğ“Ÿ-dâ‚ : (x : ğ“¢) â†’ âˆ€ {z} â†’ z âˆˆ (ğ“Ÿ x) â†’ z âŠ† x
ğ“Ÿ-dâ‚ _ = âˆ§-projâ‚ (ğ“Ÿ-d _)

ğ“Ÿ-dâ‚‚ : (x : ğ“¢) â†’ âˆ€ {z} â†’ z âŠ† x â†’ z âˆˆ (ğ“Ÿ x)
ğ“Ÿ-dâ‚‚ _ = âˆ§-projâ‚‚ (ğ“Ÿ-d _)

-- Theorem 87, p. 47 (Suppes 1960).
Aâˆˆğ“ŸA : (A : ğ“¢) â†’ A âˆˆ ğ“Ÿ A
Aâˆˆğ“ŸA A = ğ“Ÿ-dâ‚‚ A subsetOfItself

-- Theorem 91, p. 48 (Suppes 1960).
âŠ†ğ“Ÿ : (A B : ğ“¢) â†’ A âŠ† B â‡” ğ“Ÿ A âŠ† ğ“Ÿ B
âŠ†ğ“Ÿ A B = iâ‚— , iáµ£
  where
  iâ‚— : A âŠ† B â†’ ğ“Ÿ A âŠ† ğ“Ÿ B
  iâ‚— AâŠ†B t tâˆˆğ“ŸA = ğ“Ÿ-dâ‚‚ _ tâŠ†B
    where
     tâŠ†A : t âŠ† A
     tâŠ†A = ğ“Ÿ-dâ‚ A tâˆˆğ“ŸA

     tâŠ†B : t âŠ† B
     tâŠ†B = trans-âŠ† _ _ _ (tâŠ†A , AâŠ†B)
  iáµ£ : ğ“Ÿ A âŠ† ğ“Ÿ B â†’ A âŠ† B
  iáµ£ ğ“ŸAâŠ†ğ“ŸB t tâˆˆA = ğ“Ÿ-dâ‚ _ Aâˆˆğ“ŸB _ tâˆˆA
    where
    Aâˆˆğ“ŸB : A âˆˆ ğ“Ÿ B
    Aâˆˆğ“ŸB = ğ“ŸAâŠ†ğ“ŸB _ (Aâˆˆğ“ŸA _)

-- Theorem 92, p. 48 (Suppes 1960).
ğ“Ÿâˆª : (A B : ğ“¢) â†’ (ğ“Ÿ A) âˆª (ğ“Ÿ B) âŠ† ğ“Ÿ (A âˆª B)
ğ“Ÿâˆª A B t tâˆˆğ“ŸAâˆªğ“ŸB = ğ“Ÿ-dâ‚‚ _ tâŠ†AâˆªB
  where
  âˆªâ‚ : t âˆˆ ğ“Ÿ A âˆ¨ t âˆˆ ğ“Ÿ B
  âˆªâ‚ = âˆª-dâ‚ _ _ tâˆˆğ“ŸAâˆªğ“ŸB

  p : t âŠ† A âˆ¨ t âŠ† B
  p = âˆ¨-propâ‚„ auxâ‚ (ğ“Ÿ-dâ‚ _)
    where
    auxâ‚ : t âŠ† A âˆ¨ t âˆˆ ğ“Ÿ B
    auxâ‚ = âˆ¨-propâ‚ƒ âˆªâ‚ (ğ“Ÿ-dâ‚ _)
  tâŠ†AâˆªB : t âŠ† A âˆª B
  tâŠ†AâˆªB = âˆª-propâ‚‚ _ _ _ p

-- Cartesian Product. First we have to prove some things using
-- the subset axiom in order to be able to define cartesian products.

-- Two abvreviations to make subâ‚„ shorter.

abvâ‚‚ : ğ“¢ â†’ ğ“¢ â†’ ğ“¢ â†’ Set
abvâ‚‚ z A B = z âˆˆ ğ“Ÿ (ğ“Ÿ (A âˆª B))

abvâ‚ƒ : ğ“¢ â†’ ğ“¢ â†’ ğ“¢ â†’ Set
abvâ‚ƒ z A B = âˆƒ (Î» y â†’ âˆƒ (Î» w â†’ (y âˆˆ A âˆ§ w âˆˆ B) âˆ§ z â‰¡ y â‚’ w))

--Instance of the subset axiom.
subâ‚„ : (A B : ğ“¢) â†’ âˆƒ (Î» C â†’ {z : ğ“¢} â†’ z âˆˆ C â‡” abvâ‚‚ z A B âˆ§ abvâ‚ƒ z A B)
subâ‚„ A B = sub (Î» x â†’ abvâ‚ƒ x A B) (ğ“Ÿ (ğ“Ÿ (A âˆª B)))

-- Proved inside theorem 95, p. 49 (Suppes 1960)
propâ‚ : (A B x : ğ“¢) â†’ abvâ‚ƒ x A B â†’ abvâ‚‚ x A B
propâ‚ A B x (y , (z , ((yâˆˆA , zâˆˆB) , eqo))) = subs _ (sym _ _ eqo)  yâ‚’zâˆˆğ“Ÿğ“ŸAâˆªB
  where
  yâ‚›âŠ†A : singleton y âŠ† A
  yâ‚›âŠ†A = singleton-âŠ† _ _ yâˆˆA

  yâ‚›âŠ†AâˆªB : singleton y âŠ† A âˆª B
  yâ‚›âŠ†AâˆªB t tâˆˆyâ‚› = trans-âŠ† _ _ _ (yâ‚›âŠ†A , (âˆª-prop _ _)) _ tâˆˆyâ‚›

  zâ‚›âŠ†B : singleton z âŠ† B
  zâ‚›âŠ†B = singleton-âŠ† _ _ zâˆˆB

  zâ‚›âŠ†AâˆªB : singleton z âŠ† A âˆª B
  zâ‚›âŠ†AâˆªB t tâˆˆzâ‚› = trans-âŠ† _ _ _ (zâ‚›âŠ†B , âˆª-propâ‚ƒ _ _) _ tâˆˆzâ‚›

  y,zâŠ†AâˆªB : y â‚š z âŠ† A âˆª B
  y,zâŠ†AâˆªB t tâˆˆy,z = âˆª-propâ‚„ _ _ _ yâ‚›âŠ†AâˆªB zâ‚›âŠ†AâˆªB _ p
    where
    p : t âˆˆ singleton y âˆª singleton z
    p = subs (Î» w â†’ t âˆˆ w) (prop-pâ‚‚ y z) tâˆˆy,z
  yâ‚›âˆˆğ“ŸAâˆªB : singleton y âˆˆ ğ“Ÿ (A âˆª B)
  yâ‚›âˆˆğ“ŸAâˆªB = ğ“Ÿ-dâ‚‚ _ yâ‚›âŠ†AâˆªB

  y,zâˆˆğ“ŸAâˆªB : y â‚š z âˆˆ ğ“Ÿ (A âˆª B)
  y,zâˆˆğ“ŸAâˆªB = ğ“Ÿ-dâ‚‚ _ y,zâŠ†AâˆªB

  yâ‚’zâŠ†ğ“ŸAâˆªB : y â‚’ z âŠ† ğ“Ÿ (A âˆª B)
  yâ‚’zâŠ†ğ“ŸAâˆªB t tâˆˆo = âˆ¨-e _ _ _ (pair-dâ‚ _ _ tâˆˆo) iâ‚ iâ‚‚
    where
    iâ‚ : t â‰¡ singleton y â†’ t âˆˆ ğ“Ÿ (A âˆª B)
    iâ‚ eq = subs _ (sym t (singleton y) eq) yâ‚›âˆˆğ“ŸAâˆªB

    iâ‚‚ : t â‰¡ y â‚š z â†’ t âˆˆ ğ“Ÿ (A âˆª B)
    iâ‚‚ eq = subs _ (sym t (y â‚š z) eq) y,zâˆˆğ“ŸAâˆªB
  yâ‚’zâˆˆğ“Ÿğ“ŸAâˆªB : y â‚’ z âˆˆ ğ“Ÿ (ğ“Ÿ (A âˆª B))
  yâ‚’zâˆˆğ“Ÿğ“ŸAâˆªB = ğ“Ÿ-dâ‚‚ _ yâ‚’zâŠ†ğ“ŸAâˆªB

Aáµ¤ : ğ“¢ â†’ ğ“¢ â†’ ğ“¢
Aáµ¤ A B = projâ‚ (subâ‚„ A B)

-- Theorem 95, p 49 (Suppes 1960).
pAáµ¤ : (A B : ğ“¢) â†’ {z : ğ“¢} â†’ z âˆˆ (Aáµ¤ A B) â‡” abvâ‚‚ z A B âˆ§ abvâ‚ƒ z A B
pAáµ¤ A B = projâ‚‚ _ (subâ‚„ A B)

crts : (A B : ğ“¢) â†’ âˆƒ (Î» C â†’ (z : ğ“¢) â†’ z âˆˆ C â‡” abvâ‚ƒ z A B)
crts A B  = (Aáµ¤ A B) , (Î» w â†’ â‡”-pâ‚‚ w (pAáµ¤ A B) (propâ‚ A B w))

_X_ : ğ“¢ â†’ ğ“¢ â†’ ğ“¢
A X B = projâ‚ (crts A B)

-- Theorem 97, p. 50 (Suppes 1960).
crts-p : (A B x : ğ“¢) â†’ x âˆˆ A X B â‡” abvâ‚ƒ x A B
crts-p A B x = projâ‚‚ _ (crts A B) x

-- Both projections
crts-pâ‚ : (A B x : ğ“¢) â†’  x âˆˆ A X B â†’ abvâ‚ƒ x A B
crts-pâ‚ A B x = âˆ§-projâ‚ (crts-p A B x)

crts-pâ‚‚ : (A B x : ğ“¢) â†’ abvâ‚ƒ x A B â†’ x âˆˆ A X B
crts-pâ‚‚ A B x = âˆ§-projâ‚‚ (crts-p A B x)

crts-dâ‚ : (x y A B : ğ“¢) â†’ x â‚’ y âˆˆ A X B â†’ x âˆˆ A âˆ§ y âˆˆ B
crts-dâ‚ x y A B h = (subs (Î» w â†’ w âˆˆ A) (sym _ _ eqâ‚) auxâˆˆA)
                         ,
                         subs (Î» w â†’ w âˆˆ B) (sym _ _ eqâ‚‚) auxâ‚‚âˆˆB
  where
  foo : âˆƒ (Î» z â†’ âˆƒ (Î» w â†’ (z âˆˆ A âˆ§ w âˆˆ B) âˆ§ (x â‚’ y) â‰¡ (z â‚’ w)))
  foo = crts-pâ‚ A B (x â‚’ y) h

  aux : ğ“¢
  aux = projâ‚ foo

  aux-p : âˆƒ (Î» w â†’ (aux âˆˆ A âˆ§ w âˆˆ B) âˆ§ (x â‚’ y) â‰¡ (aux â‚’ w))
  aux-p = projâ‚‚ _ foo

  auxâ‚‚ : ğ“¢
  auxâ‚‚ = projâ‚ aux-p

  auxâ‚‚-p : (aux âˆˆ A âˆ§ auxâ‚‚ âˆˆ B) âˆ§ (x â‚’ y) â‰¡ (aux â‚’ auxâ‚‚)
  auxâ‚‚-p = projâ‚‚ _ aux-p

  auxâˆˆA : aux âˆˆ A
  auxâˆˆA = âˆ§-projâ‚ (âˆ§-projâ‚ auxâ‚‚-p)

  auxâ‚‚âˆˆB : auxâ‚‚ âˆˆ B
  auxâ‚‚âˆˆB = âˆ§-projâ‚‚ (âˆ§-projâ‚ auxâ‚‚-p)

  eq : x â‚’ y â‰¡ aux â‚’ auxâ‚‚
  eq = âˆ§-projâ‚‚ auxâ‚‚-p

  eqs : x â‰¡ aux âˆ§ y â‰¡ auxâ‚‚
  eqs = ord-p _ _ _ _ eq

  eqâ‚ : x â‰¡ aux
  eqâ‚ = âˆ§-projâ‚ eqs

  eqâ‚‚ : y â‰¡ auxâ‚‚
  eqâ‚‚ = âˆ§-projâ‚‚ eqs

-- References
--
-- Suppes, Patrick (1960). Axiomatic Set Theory.
-- The University Series in Undergraduate Mathematics.
-- D. Van Nostrand Company, inc.
--
-- Enderton, Herbert B. (1977). Elements of Set Theory.
-- Academic Press Inc.
