------------------------------------------
-- Set theory formalization
------------------------------------------

module SetTheory where

infix 6 _-_
infix 6 _âˆ©_
infix 6 _â‚š_
infix 6 _âˆª_
infix 5 _âŠ†_
infix 5 _âˆˆ_ _âˆ‰_
infix 4 _â‰¡_
infix 4 _,_
infix 3 Â¬_
infix 2 _âˆ§_
infix 2 âˆƒ
infix 1 _âˆ¨_
infix 0 _â‡”_


-- 0ur Sets will be called denoted by ğ“¢. This is
-- our universe of discourse. Membership of set
-- is also a primitive notion. That letter is
-- written by "\MCS"

postulate
  ğ“¢   : Set
  _âˆˆ_ : ğ“¢ â†’ ğ“¢ â†’ Set

------------------------------------------
-- Some First order logic I need.

-- âˆ§ data type (conjunction).

data _âˆ§_ (A B : Set) : Set where
  _,_ : A â†’ B â†’ A âˆ§ B

âˆ§-projâ‚ : âˆ€ {A B} â†’ A âˆ§ B â†’ A
âˆ§-projâ‚ (a , _) = a

âˆ§-projâ‚‚ : âˆ€ {A B} â†’ A âˆ§ B â†’ B
âˆ§-projâ‚‚ (_ , b) = b

-- âˆ¨ data type (disjunction).

data _âˆ¨_ (A B : Set) : Set where
  injâ‚ : A â†’ A âˆ¨ B
  injâ‚‚ : B â†’ A âˆ¨ B

âˆ¨-e : (A B C : Set) â†’ A âˆ¨ B â†’ (A â†’ C) â†’ (B â†’ C) â†’ C
âˆ¨-e A B C (injâ‚ a) iâ‚ iâ‚‚ = iâ‚ a
âˆ¨-e A B C (injâ‚‚ b) iâ‚ iâ‚‚ = iâ‚‚ b

trivial : (A : Set) â†’ A â†’ A
trivial _ A = A

âˆ¨-idem : (A : Set) â†’ A âˆ¨ A â†’ A
âˆ¨-idem A (injâ‚ a) = a
âˆ¨-idem A (injâ‚‚ a) = a

-- Bi-implication.

_â‡”_ : Set â†’ Set â†’ Set
A â‡” B = (A â†’ B) âˆ§ (B â†’ A)

-- Empty data type.

data âŠ¥ : Set where

âŠ¥-elim : {A : Set} â†’ âŠ¥ â†’ A
âŠ¥-elim ()

-- Negation

Â¬_ : Set â†’ Set
Â¬ A = A â†’ âŠ¥

-- Existential quantifier

data âˆƒ (A : ğ“¢ â†’ Set) : Set where
  _,_ : (t : ğ“¢) â†’ A t â†’ âˆƒ A

-- Sugar syntax for the existential quantifier.

syntax âˆƒ (Î» x â†’ e) = âˆƒ[ x ] e

-- Existential projection.

projâ‚ : {A : ğ“¢ â†’ Set} â†’ âˆƒ A â†’ ğ“¢
projâ‚ (t , _) = t

projâ‚‚ : (A : ğ“¢ â†’ Set) â†’ (foo : âˆƒ A)  â†’ A (projâ‚ foo)
projâ‚‚ A (_ , Ax) = Ax

-------------------------------------------

-- Equivalence and non equivalence

data _â‰¡_ (x : ğ“¢) : ğ“¢ â†’ Set where
  refl : x â‰¡ x

_â‰¢_ : ğ“¢ â†’ ğ“¢ â†’ Set
x â‰¢ y = Â¬ x â‰¡ y

sym : (x y : ğ“¢) â†’ x â‰¡ y â†’ y â‰¡ x
sym x .x refl = refl

cong : (f : â€„ğ“¢ â†’ ğ“¢) {x y : ğ“¢} â†’ x â‰¡ y â†’ f x â‰¡ f y
cong f refl = refl

subs : (P : ğ“¢ â†’ Set) {x y : ğ“¢} (p : x â‰¡ y) (h : P x) â†’ P y
subs P {x} {.x} refl h = h


-- Definitions of subset and not-membership.

_âŠ†_ : ğ“¢ â†’ ğ“¢ â†’ Set
x âŠ† y = (t : ğ“¢) â†’ t âˆˆ x â†’ t âˆˆ y

_âˆ‰_ : ğ“¢ â†’ ğ“¢ â†’ Set
x âˆ‰ y = Â¬ (x âˆˆ y)
{-# ATP definition _âˆ‰_ #-}

_âŠ‚_ : ğ“¢ â†’ ğ“¢ â†’ Set
x âŠ‚ y = x âŠ† y âˆ§ x â‰¢ y

_âŠ‚'_ : ğ“¢ â†’ ğ“¢ â†’ Set
x âŠ‚' y = x âŠ† y âˆ§ âˆƒ (Î» z â†’ z âˆˆ y âˆ§ z âˆ‰ x)


-------------------------------------------

-- The Axioms

-- ext (Extensionality) : If two sets have exactly the same members,
-- they are equal.  empt (Empty Set Axiom) : There is a set having no
-- members.


-- pair (Pairing Axiom) : For any sets y and z, there is a set having
-- as members just y and z.

-- pow (Power Set Axiom): For any x there is a set whose members are
-- exactly the subsets of x.

-- sub (Subset Axiom, or Specification Axiom): This axiom asserts the
-- existence of a set B whose members are exactly those sets x in y
-- such that they satisfy certain property.

-- uni (Union Axiom) : For any set x, there exists a set A whose
-- elements are exactly the members of x.

-- The other three axioms are yet to implement.

postulate
  ext  : (x y : ğ“¢) â†’ âˆ€ {z} â†’ z âˆˆ x â‡” z âˆˆ y â†’ x â‰¡ y
  union : (x y : ğ“¢) â†’ âˆƒ (Î» B â†’ {z : ğ“¢} â†’ z âˆˆ B â‡” z âˆˆ x âˆ¨ z âˆˆ y)
  pair : (x y : ğ“¢) â†’ âˆƒ (Î» B â†’ {z : ğ“¢} â†’ z âˆˆ B â‡” (z â‰¡ x âˆ¨ z â‰¡ y))
  pow : âˆ€ {x} â†’ âˆƒ (Î» B â†’ âˆ€ {y} â†’ y âˆˆ B â‡” y âŠ† x)
  sub  : (A : ğ“¢ â†’ Set) â†’ (y : ğ“¢) â†’ âˆƒ (Î» B â†’ (x : ğ“¢) â†’ (x âˆˆ B â‡” (x âˆˆ y âˆ§ A x)))
{-# ATP axioms ext union #-}
  -- uni  : âˆ€ {z} â†’ (âˆƒ A : ğ“¢) â†’ âˆ€ {y x} â†’ x âˆˆ y âˆ§ y âˆˆ z â†’ x âˆˆ A
------------------------------------------

-- Pairs, singletons.

_â‚š_ : ğ“¢ â†’ ğ“¢ â†’ ğ“¢
x â‚š y = projâ‚ (pair x y)

singleton : ğ“¢ â†’ ğ“¢
singleton x = x â‚š x


postulate
  empt : âˆƒ (Î» B â†’ âˆ€ x â†’ x âˆ‰ B)
{-# ATP axioms empt #-}

âˆ… : ğ“¢
âˆ… = projâ‚ empt
{-# ATP definition âˆ… #-}

notInEmpty : âˆ€ x â†’ x âˆ‰ âˆ…
notInEmpty x h  = (projâ‚‚ _ empt) x h

-- I am having troubles proving this theorem (unique-âˆ…).
-- The left hand side of the implication is easily provable,
-- but the right side is not. I tried seeing if apia could prove it,
-- but it couldn't either.

-- postulate unique-âˆ… : (x y : ğ“¢) â†’ ((x âˆ‰ y) â‡” y â‰¡ âˆ…)
-- {-# ATP prove unique-âˆ… #-}

subsetOfItself : âˆ€ {x} â†’ x âŠ† x
subsetOfItself _ tâˆˆx = tâˆˆx

equalitySubset :  (x y : ğ“¢) â†’ x âŠ† y âˆ§ y âŠ† x â†’ x â‰¡ y
equalitySubset x y (xâŠ†y , yâŠ†x) = ext x y ((xâŠ†y x) , (yâŠ†x x))

-- This theorem depends on the proof of unique-âˆ… so I didn't prove it.
-- postulate subsetOf-âˆ… : (x : â€„ğ“¢) (p : x âŠ† âˆ…) â†’ x â‰¡ âˆ…
-- {-# ATP prove subsetOf-âˆ… #-}

trans-âŠ† : (x y z : ğ“¢) â†’ x âŠ† y âˆ§ y âŠ† z â†’ x âŠ† z
trans-âŠ† x y z (xâŠ†y , yâŠ†z) t tâˆˆx = yâŠ†z t (xâŠ†y t tâˆˆx)

notContainedInItself : âˆ€ {x} â†’ Â¬ (x âŠ‚ x)
notContainedInItself (_ , xâ‰¢x) = xâ‰¢x refl

nonSymmetry-âŠ‚ : (x y : ğ“¢) (p : x âŠ‚ y) â†’ Â¬ (y âŠ‚ x)
nonSymmetry-âŠ‚ x y (xâŠ†y , xâ‰¢y) (yâŠ†x , _) = xâ‰¢y (equalitySubset x y (xâŠ†y , yâŠ†x))

âŠ‚â†’âŠ† : âˆ€ {x y} â†’ x âŠ‚ y â†’ x âŠ† y
âŠ‚â†’âŠ† (xâŠ†y , _) z zâˆˆx = xâŠ†y z zâˆˆx

_âˆ©_ : ğ“¢ â†’ ğ“¢ â†’ ğ“¢
x âˆ© y = projâ‚ (sub (Î» z â†’ z âˆˆ x) y)

_âˆª_ : ğ“¢ â†’ ğ“¢ â†’ ğ“¢
x âˆª y = projâ‚ (union x y)
{-# ATP definition _âˆª_ #-}

-- projâ‚‚ : (A : ğ“¢ â†’ Set) â†’ (foo : âˆƒ A)  â†’ A (projâ‚ foo)
-- projâ‚‚ A (_ , Ax) = Ax
-- union : (x y : ğ“¢) â†’ âˆƒ (Î» B â†’ âˆ€ {z} â†’ z âˆˆ B â‡” z âˆˆ x âˆ¨ z âˆˆ y)

theorem : (x y : ğ“¢) â†’ âˆ€ {z} â†’ z âˆˆ x âˆª y â‡” z âˆˆ x âˆ¨ z âˆˆ y
theorem x y = projâ‚‚ _ (union x y)


postulate
 âˆª-d : (x A B : ğ“¢) â†’ x âˆˆ (A âˆª B) â‡” x âˆˆ A âˆ¨ x âˆˆ B
 âˆ©-def : (x A B : ğ“¢) â†’ x âˆˆ (A âˆ© B) â‡” x âˆˆ A âˆ§ x âˆˆ B
{-# ATP prove âˆª-d #-}

âˆ©-dâ‚ : (x A B : ğ“¢)  â†’ x âˆˆ (A âˆ© B) â†’ x âˆˆ A âˆ§ x âˆˆ B
âˆ©-dâ‚ x A B = âˆ§-projâ‚ (âˆ©-def x A B)

âˆ©-dâ‚‚ : (x A B : ğ“¢) â†’ x âˆˆ A âˆ§ x âˆˆ B â†’ x âˆˆ (A âˆ© B)
âˆ©-dâ‚‚ x A B = âˆ§-projâ‚‚ (âˆ©-def x A B)

âˆ©-sym : (A B : ğ“¢) â†’ A âˆ© B â‰¡ B âˆ© A
âˆ©-sym A B = equalitySubset (A âˆ© B) (B âˆ© A) (pâ‚ , pâ‚‚)
  where
  pâ‚ : (x : ğ“¢) â†’ x âˆˆ A âˆ© B â†’ x âˆˆ B âˆ© A
  pâ‚ x xâˆˆAâˆ©B = âˆ©-dâ‚‚ x B A (xâˆˆB , xâˆˆA)
    where
    xâˆˆA : x âˆˆ A
    xâˆˆA = âˆ§-projâ‚ (âˆ©-dâ‚ x A B xâˆˆAâˆ©B)
    xâˆˆB : x âˆˆ B
    xâˆˆB = âˆ§-projâ‚‚ (âˆ©-dâ‚ x A B xâˆˆAâˆ©B)
  pâ‚‚ : (x : â€¯ğ“¢) â†’ x âˆˆ B âˆ© A â†’ x âˆˆ A âˆ© B
  pâ‚‚ x xâˆˆBâˆ©A = âˆ©-dâ‚‚ x A B (xâˆˆA , xâˆˆB)
    where
    xâˆˆA : x âˆˆ A
    xâˆˆA = âˆ§-projâ‚‚ (âˆ©-dâ‚ x B A xâˆˆBâˆ©A)
    xâˆˆB : x âˆˆ B
    xâˆˆB = âˆ§-projâ‚ (âˆ©-dâ‚ x B A xâˆˆBâˆ©A)

âˆ©-dist : (A B C : ğ“¢) â†’ (A âˆ© B) âˆ© C â‰¡ A âˆ© (B âˆ© C)
âˆ©-dist A B C = equalitySubset ((A âˆ© B) âˆ© C) (A âˆ© (B âˆ© C)) (pâ‚ , pâ‚‚)
  where
  pâ‚ : (x : ğ“¢) â†’ x âˆˆ (A âˆ© B) âˆ© C â†’ x âˆˆ A âˆ© (B âˆ© C)
  pâ‚ x xâ‚ = âˆ©-dâ‚‚ x A (B âˆ© C) (xâˆˆA , xâˆˆBâˆ©C)
    where
    xâˆˆBâˆ©C : x âˆˆ B âˆ© C
    xâˆˆBâˆ©C = âˆ©-dâ‚‚ x B C (xâˆˆB , xâˆˆC)
      where
      xâˆˆAâˆ©B : x âˆˆ A âˆ© B
      xâˆˆAâˆ©B = âˆ§-projâ‚ (âˆ©-dâ‚ x (A âˆ© B) _ xâ‚)
      xâˆˆB : x âˆˆ B
      xâˆˆB = âˆ§-projâ‚‚ (âˆ©-dâ‚ x _ B xâˆˆAâˆ©B)
      xâˆˆC : x âˆˆ C
      xâˆˆC = âˆ§-projâ‚‚ (âˆ©-dâ‚ x _ C xâ‚)
    xâˆˆA : x âˆˆ A
    xâˆˆA = âˆ§-projâ‚ (âˆ©-dâ‚ x A _ xâˆˆAâˆ©B)
      where
      xâˆˆAâˆ©B : x âˆˆ A âˆ© B
      xâˆˆAâˆ©B = âˆ§-projâ‚ (âˆ©-dâ‚ x (A âˆ© B) _ xâ‚)
  pâ‚‚ : (x : ğ“¢) â†’ x âˆˆ A âˆ© (B âˆ© C) â†’ x âˆˆ (A âˆ© B) âˆ© C
  pâ‚‚ x xâ‚ = âˆ©-dâ‚‚ x (A âˆ© B) C (xâˆˆAâˆ©B , xâˆˆC)
    where
    xâˆˆAâˆ©B : x âˆˆ A âˆ© B
    xâˆˆAâˆ©B = âˆ©-dâ‚‚ x A B (xâˆˆA , xâˆˆB)
      where
      xâˆˆA : x âˆˆ A
      xâˆˆA = âˆ§-projâ‚ (âˆ©-dâ‚ x A _ xâ‚)
      xâˆˆBâˆ©C : x âˆˆ B âˆ© C
      xâˆˆBâˆ©C = âˆ§-projâ‚‚ (âˆ©-dâ‚ x _ (B âˆ© C) xâ‚)
      xâˆˆB : x âˆˆ B
      xâˆˆB = âˆ§-projâ‚ (âˆ©-dâ‚ x B _ xâˆˆBâˆ©C)
    xâˆˆC : x âˆˆ C
    xâˆˆC = âˆ§-projâ‚‚ (âˆ©-dâ‚ x _ C xâˆˆBâˆ©C)
      where
      xâˆˆBâˆ©C : x âˆˆ B âˆ© C
      xâˆˆBâˆ©C = âˆ§-projâ‚‚ (âˆ©-dâ‚ x _ (B âˆ© C) xâ‚)

âˆ©-itself : (A : ğ“¢) â†’ A âˆ© A â‰¡ A
âˆ©-itself A = equalitySubset (A âˆ© A) A (pâ‚ , pâ‚‚)
  where
  pâ‚ : (x : ğ“¢) â†’ x âˆˆ A âˆ© A â†’ x âˆˆ A
  pâ‚ x xâ‚ = âˆ§-projâ‚ (âˆ©-dâ‚ _ A _ xâ‚)
  pâ‚‚ : (x : â€„ğ“¢) â†’ x âˆˆ A â†’ x âˆˆ A âˆ© A
  pâ‚‚ x xâ‚ = âˆ©-dâ‚‚ _ A A (xâ‚ , xâ‚)

Aâˆ©BâŠ†A : (A B : ğ“¢) â†’ A âˆ© B âŠ† A
Aâˆ©BâŠ†A A B _ p = âˆ§-projâ‚ (âˆ©-dâ‚ _ A _ p)

âˆª-dâ‚ : (x A B : ğ“¢) â†’ x âˆˆ (A âˆª B) â†’ x âˆˆ A âˆ¨ x âˆˆ B
âˆª-dâ‚ x A B = âˆ§-projâ‚ (âˆª-d x A B)

âˆª-dâ‚‚ : (x A B : ğ“¢) â†’ x âˆˆ A âˆ¨ x âˆˆ B â†’ x âˆˆ (A âˆª B)
âˆª-dâ‚‚ x A B = âˆ§-projâ‚‚ (âˆª-d x A B)

postulate
 pair-d : (x y z : ğ“¢) â†’ z âˆˆ (x â‚š y) â‡” z â‰¡ x âˆ¨ z â‰¡ y

-- th : âˆ€ {z} â†’ (x y : ğ“¢) â†’ z âˆˆ x â‚š y â‡” z â‰¡ x âˆ¨ x â‰¡ y
-- th x y = projâ‚‚ (Î» z â†’ z âˆˆ x â‚š y â‡” z â‰¡ x âˆ¨ z â‰¡ y) {!!}

_-_ : ğ“¢ â†’ ğ“¢ â†’ ğ“¢
x - y = projâ‚ (sub (Î» z â†’ z âˆ‰ x) y)

postulate
 dif-d : (A B z : ğ“¢) â†’ z âˆˆ A - B â‡” z âˆˆ A âˆ§ z âˆ‰ B

dif-dâ‚ : (A B z : ğ“¢) â†’ z âˆˆ A - B â†’ z âˆˆ A âˆ§ z âˆ‰ B
dif-dâ‚ A B z = âˆ§-projâ‚ (dif-d A B z)

dif-dâ‚‚ : (A B z : ğ“¢) â†’ z âˆˆ A âˆ§ z âˆ‰ B â†’ z âˆˆ A - B
dif-dâ‚‚ A B z = âˆ§-projâ‚‚ (dif-d A B z)

âˆ©- : (A B : ğ“¢) â†’ A âˆ© (A - B) â‰¡ A - B
âˆ©- A B = equalitySubset (A âˆ© (A - B)) (A - B) (pâ‚ , pâ‚‚)
  where
  pâ‚ : (x : ğ“¢) â†’ x âˆˆ A âˆ© (A - B) â†’ x âˆˆ A - B
  pâ‚ x xâˆˆâˆ©- = dif-dâ‚‚ A B x (xâˆˆA , xâˆ‰B)
    where
    xâˆˆA : x âˆˆ A
    xâˆˆA = âˆ§-projâ‚ (âˆ©-dâ‚ x A _ xâˆˆâˆ©-)
    xâˆˆA-B : x âˆˆ A - B
    xâˆˆA-B = âˆ§-projâ‚‚ (âˆ©-dâ‚ x _ (A - B) xâˆˆâˆ©-)
    xâˆ‰B : x âˆ‰ B
    xâˆ‰B = âˆ§-projâ‚‚ (dif-dâ‚ A B x xâˆˆA-B)
  pâ‚‚ : (x : ğ“¢) â†’ x âˆˆ A - B â†’ x âˆˆ A âˆ© (A - B)
  pâ‚‚ x xâˆˆA-B = âˆ©-dâ‚‚ x A (A - B) ((âˆ§-projâ‚ (dif-dâ‚ A B x xâˆˆA-B)) , xâˆˆA-B)
